src/program_proof/map_string_marshal_proof.v
@@ -1,0 +1,179 @@
+From Perennial.program_proof Require Import grove_prelude marshal_stateless_proof.
+From Perennial.goose_lang.lib Require Import typed_map map.impl.
+From Goose.github_com.mit_pdos.gokv Require Import map_string_marshal.
+
+Section map_string_marshal_proof.
+
+Context `{!heapGS Σ}.
+
+Local Definition encode_maplist (l:list (string * string)) : list u8 :=
+  flat_map (λ u,
+              (u64_le (int.Z (length (string_to_bytes u.1)))) ++
+              (string_to_bytes u.1) ++
+              (u64_le (int.Z (length (string_to_bytes u.2)))) ++
+              (string_to_bytes u.2)) l.
+
+Local Lemma encode_maplist_cons k data l :
+  encode_maplist ((k, data)::l) =
+              ((u64_le $ int.Z $ length $ string_to_bytes k) ++
+               (string_to_bytes k) ++
+               (u64_le $ int.Z $ length $ string_to_bytes data) ++
+               (string_to_bytes data)) ++ encode_maplist l.
+Proof. done. Qed.
+
+Local Definition has_partial_map_encoding (enc:list u8) (fullsize: u64) (m:gmap string string) : Prop :=
+  ∃ l,
+  NoDup l.*1 ∧
+  (list_to_map l) = m ∧
+  enc = (u64_le fullsize) ++ encode_maplist l.
+
+Definition has_string_map_encoding (enc:list u8) (m:gmap string string) : Prop :=
+  int.Z (size m) = size m ∧ has_partial_map_encoding enc (size m) m.
+
+Lemma wp_EncodeStringMap mptr m :
+  {{{
+        "Hmap" ∷ own_map mptr 1 m
+  }}}
+    EncodeStringMap #mptr
+  {{{
+        enc_sl enc, RET (slice_val enc_sl);
+        own_map mptr 1 m ∗
+        own_slice enc_sl byteT 1 enc ∗
+        ⌜has_string_map_encoding enc m⌝
+  }}}.
+Proof.
+  iIntros "%Φ H HΦ". iNamed "H". iNamed "Hmap". wp_call.
+  wp_apply wp_NewSlice. iIntros (s) "Hs".
+  wp_apply wp_ref_to; first by val_ty. iIntros (l) "Hl".
+  (*
+  wp_apply (wp_MapLen with "Hkvs_map"). iIntros "[%Hmsize Hkvs_map]".
+  wp_load.
+  wp_apply (wp_WriteInt with "Hs"). iIntros (s') "Hs".
+  rewrite replicate_0 /=. wp_store. clear s.
+  wp_apply (wp_MapIter_2 _ _ _ _ _
+    (λ kvs_todo kvs_done, ∃ (s : Slice.t) enc,
+      "%Hm" ∷ ⌜kvs_sl = kvs_todo ∪ kvs_done⌝ ∗
+      "%Hdisk" ∷ ⌜dom kvs_todo ## dom kvs_done⌝ ∗
+      "%Henc" ∷ ⌜has_partial_byte_map_encoding enc (size m) (map_zip_with (λ v _, v) m kvs_done)⌝ ∗
+      "Hl" ∷ l ↦[slice.T byteT] (slice_val s) ∗
+      "Hs" ∷ own_slice s byteT 1 enc
+    )%I with "Hkvs_map [Hl Hs]").
+  { iExists _, _. iFrame. iPureIntro.
+    rewrite right_id_L. split; first done.
+    rewrite /has_partial_byte_map_encoding.
+    split; first set_solver.
+    exists [].
+    split; first by apply NoDup_nil_2.
+    rewrite map_zip_with_empty_r.
+    split; first by apply list_to_map_nil.
+    do 2 rewrite -size_dom. rewrite -Hkvs_dom size_dom. done. }
+  { (* core loop *)
+     clear Φ s' mptr. iIntros (k v kvs_todo kvs_done Φ) "!# [HI %Hk] HΦ". iNamed "HI". wp_pures.
+     wp_load. wp_apply (wp_WriteInt with "Hs"). iIntros (s') "Hs". wp_store. clear s.
+     wp_apply wp_slice_len.
+     wp_load. wp_apply (wp_WriteInt with "Hs"). iIntros (s) "Hs". wp_store. clear s'.
+     iSpecialize ("Hkvs_slices" $! k).
+     iMod (readonly_load with "Hkvs_slices") as (q) "Hk".
+     iDestruct (own_slice_small_sz with "Hk") as %Hsz.
+     iEval (rewrite Hm) in "Hk".
+     erewrite lookup_union_Some_l by done. simpl.
+     wp_load. wp_apply (wp_WriteBytes with "[$Hs $Hk]"). iIntros (s') "[Hs _]". wp_store. clear s.
+     iApply "HΦ". iModIntro. iExists _, _. iFrame. iPureIntro.
+     split.
+     { rewrite union_delete_insert //. }
+     assert (kvs_done !! k = None).
+     { apply not_elem_of_dom. apply elem_of_dom_2 in Hk. set_solver. }
+     split; first set_solver.
+     assert (is_Some (m !! k)) as [data Hdata].
+     { apply elem_of_dom. rewrite -Hkvs_dom Hm dom_union. apply elem_of_dom_2 in Hk. set_solver. }
+     destruct Henc as (ls & Hnodup & Hls & Henc). exists (ls ++ [(k, data)]).
+     assert (k ∉ ls.*1).
+     { intros Hin. eapply (not_elem_of_list_to_map ls). 2:by apply Hin.
+       rewrite Hls. apply map_lookup_zip_with_None. auto. }
+     split; last split.
+     - rewrite fmap_app. apply NoDup_app. split; first done.
+       simpl. split; last by apply NoDup_singleton.
+       intros k' Hk' ->%elem_of_list_singleton. done.
+     - rewrite list_to_map_snoc //. rewrite Hls.
+       change data with ((λ v _, v) data v).
+       rewrite map_insert_zip_with. rewrite insert_id //.
+     - rewrite Hdata Henc. cbn. rewrite -!app_assoc. repeat f_equal.
+       rewrite /encode_byte_maplist flat_map_app. f_equal. cbn. rewrite -!app_assoc app_nil_r. repeat f_equal.
+       move:Hsz. rewrite Hdata Hm. erewrite lookup_union_Some_l by done. cbn. intros. word.
+  }
+  iIntros "[Hkvs_map HI]". iNamed "HI".
+  wp_load. iApply "HΦ". iFrame. iSplitL.
+  { iExists _. iFrame. eauto. }
+  iPureIntro. split.
+  - rewrite -size_dom -Hkvs_dom size_dom. rewrite Hmsize. word.
+  - replace m with (map_zip_with (λ (v : list u8) (_ : Slice.t), v) m kvs_sl) at 2. 1:done.
+    clear Henc. rewrite -[map_zip_with _ _ _]map_fmap_id. rewrite map_fmap_zip_with_l; auto.
+    intros k. rewrite -!elem_of_dom. set_solver. *)
+Admitted.
+
+Lemma wp_DecodeStringMap enc_sl enc enc_rest q m :
+  {{{
+        "%Henc" ∷ ⌜has_string_map_encoding enc m⌝ ∗
+        "Henc_sl" ∷ own_slice_small enc_sl byteT q (enc ++ enc_rest)
+  }}}
+    DecodeStringMap (slice_val enc_sl)
+  {{{
+        mptr, RET #mptr; own_map mptr 1 m
+  }}}.
+Proof.
+  iIntros "%Φ H HΦ". iNamed "H". wp_call.
+  wp_apply wp_ref_to; first by val_ty. iIntros (l) "Hl".
+  (*
+  wp_apply wp_byteMapNew. iIntros (mptr) "Hm".
+  wp_load.
+  destruct Henc as [Hsz (ls & Hnodup & Hls & Henc)]. subst enc.
+  rewrite -!app_assoc.
+  wp_apply (wp_ReadInt with "Henc_sl"). iIntros (s') "Hs". wp_store. clear enc_sl.
+  wp_apply wp_ref_to; first by val_ty. iIntros (li) "Hli". wp_pures.
+  wp_apply (wp_forUpto (λ i, ∃ s,
+              "Hm" ∷ own_byte_map mptr (list_to_map (take (int.nat i) ls)) ∗
+              "Hl" ∷ l ↦[slice.T byteT] (slice_val s) ∗
+              "Hs" ∷ own_slice_small s byteT q (encode_byte_maplist (drop (int.nat i) ls) ++ enc_rest)
+  )%I with "[] [$Hli Hm Hl Hs]"); first word.
+  2:{ iExists _. iFrame. }
+  { (* core loop *)
+    clear s' Φ. iIntros (i Φ) " !#(I & Hli & %Hi) HΦ". iNamed "I". wp_lam.
+    replace (int.nat (u64_instance.u64.(word.add) i 1)) with (1 + int.nat i)%nat by word.
+    assert (is_Some (ls !! (int.nat i))) as [[k data] Hk].
+    { apply lookup_lt_is_Some_2. rewrite -Map.size_list_to_map //.
+      rewrite Hls. word. }
+    rewrite -(take_drop_middle _ _ _ Hk) in Hls Hnodup.
+    move:Hnodup. clear Hls.
+    erewrite take_S_r by done.
+    rewrite (drop_S _ _ _ Hk).
+    set ls_head := take (int.nat i) ls.
+    set ls_tail := drop (1+int.nat i) ls.
+    intros Hnodup.
+    rewrite encode_byte_maplist_cons -!app_assoc.
+    wp_load.
+    wp_apply (wp_ReadInt with "Hs"). iIntros (s') "Hs".
+    wp_apply (wp_ReadInt with "Hs"). iIntros (s'') "Hs".
+    iDestruct (own_slice_small_sz with "Hs") as %Hdatasz.
+    wp_apply (wp_ReadBytesCopy with "Hs").
+    { rewrite !app_length in Hdatasz. word. }
+    iIntros (sl s''') "[Hval Hs]". wp_store. clear s s' s'' Hdatasz.
+    wp_apply (wp_byteMapPut with "[$Hm Hval]").
+    { iDestruct (own_slice_to_small with "Hval") as "$". }
+    iIntros "Hm". wp_pures. iApply "HΦ". iModIntro.
+    iFrame "Hli". iExists _. iFrame. iExactEq "Hm". rewrite /named. f_equal.
+    rewrite list_to_map_snoc //.
+    rewrite fmap_app NoDup_app in Hnodup.
+    destruct Hnodup as (_ & Hnin & _). intros Hin. eapply Hnin; first done.
+    eapply elem_of_list_fmap_1_alt.
+    - apply elem_of_list_here.
+    - done. }
+  iIntros "(I & Hli)". iNamed "I". wp_load. wp_pures. iApply "HΦ". iModIntro.
+  rewrite take_ge.
+  2:{ rewrite -Map.size_list_to_map // Hls. word. }
+  rewrite Hls. iFrame "Hm".
+  rewrite drop_ge.
+  2:{ rewrite -Map.size_list_to_map // Hls. word. }
+  done. *)
+Admitted.
+
+End map_string_marshal_proof.
